<?xml version="1.0"?>
<rdf:RDF xmlns="https://purl.org/samcore#"
     xml:base="https://purl.org/samcore"
     xmlns:dc="http://purl.org/dc/terms/"
     xmlns:owl="http://www.w3.org/2002/07/owl#"
     xmlns:rdf="http://www.w3.org/1999/02/22-rdf-syntax-ns#"
     xmlns:wdp="https://www.wikidata.org/wiki/Property:"
     xmlns:wdt="https://www.wikidata.org/wiki/"
     xmlns:xml="http://www.w3.org/XML/1998/namespace"
     xmlns:xsd="http://www.w3.org/2001/XMLSchema#"
     xmlns:cwrc="https://sparql.cwrc.ca/ontologies/cwrc.html#"
     xmlns:rdfs="http://www.w3.org/2000/01/rdf-schema#"
     xmlns:relationship="https://vocab.org/relationship/#">
    <owl:Ontology rdf:about="https://purl.org/samcore#">
        <dc:creator>Francesco Alaimo</dc:creator>
        <rdfs:comment>In this model the intention is to abstract the Story entity from any constraint given by any form of expression or carrier, using it only as the source and reference to build the Story graph, and disambiguating any definition that identify the carrier and the Abstract Story as the same object.</rdfs:comment>
        <rdfs:label>Sam (Story Abstract Metadata)</rdfs:label>
        <rdfs:label>Story</rdfs:label>
    </owl:Ontology>
    


    <!-- 
    ///////////////////////////////////////////////////////////////////////////////////////
    //
    // Annotation properties
    //
    ///////////////////////////////////////////////////////////////////////////////////////
     -->

    


    <!-- http://purl.org/dc/terms/creator -->

    <owl:AnnotationProperty rdf:about="http://purl.org/dc/terms/creator"/>
    


    <!-- http://www.w3.org/1999/02/22-rdf-syntax-ns#Description -->

    <owl:AnnotationProperty rdf:about="http://www.w3.org/1999/02/22-rdf-syntax-ns#Description"/>
    


    <!-- 
    ///////////////////////////////////////////////////////////////////////////////////////
    //
    // Object Properties
    //
    ///////////////////////////////////////////////////////////////////////////////////////
     -->

    


    <!-- https://purl.org/samcore#diegeticTime -->

    <owl:ObjectProperty rdf:about="https://purl.org/samcore#diegeticTime">
        <rdfs:domain rdf:resource="https://www.wikidata.org/wiki/Q617332"/>
        <rdfs:range rdf:resource="https://www.wikidata.org/wiki/Q12322185"/>
        <rdfs:comment>This property describes the diegetic time of a setting.</rdfs:comment>
        <rdfs:label>diegetic time</rdfs:label>
    </owl:ObjectProperty>
    


    <!-- https://purl.org/samcore#hasChange -->

    <owl:ObjectProperty rdf:about="https://purl.org/samcore#hasChange">
        <rdfs:domain rdf:resource="https://purl.org/samcore#Scene"/>
        <rdfs:range rdf:resource="https://www.wikidata.org/wiki/Q1150070"/>
        <rdfs:comment>This property links a Scene to a Change that happens in it.</rdfs:comment>
        <rdfs:label>has change</rdfs:label>
    </owl:ObjectProperty>
    


    <!-- https://purl.org/samcore#hasPlace -->

    <owl:ObjectProperty rdf:about="https://purl.org/samcore#hasPlace">
        <rdfs:domain rdf:resource="https://www.wikidata.org/wiki/Q617332"/>
        <rdfs:range rdf:resource="https://www.wikidata.org/wiki/Q17334923"/>
        <rdfs:comment>This property links a Setting to a physical location class.</rdfs:comment>
        <rdfs:label>has place</rdfs:label>
    </owl:ObjectProperty>
    


    <!-- https://purl.org/samcore#hasSetting -->

    <owl:ObjectProperty rdf:about="https://purl.org/samcore#hasSetting">
        <rdfs:domain rdf:resource="https://purl.org/samcore#Scene"/>
        <rdfs:range rdf:resource="https://www.wikidata.org/wiki/Q617332"/>
        <rdfs:comment>This property links a Scene to a correspondent Setting.</rdfs:comment>
        <rdfs:label>has setting</rdfs:label>
    </owl:ObjectProperty>
    


    <!-- https://purl.org/samcore#hasTrope -->

    <owl:ObjectProperty rdf:about="https://purl.org/samcore#hasTrope">
        <rdfs:domain rdf:resource="https://purl.org/samcore#GroupOfCharacters"/>
        <rdfs:domain rdf:resource="https://purl.org/samcore#SequenceOfScenes"/>
        <rdfs:domain rdf:resource="https://purl.org/samcore#Story"/>
        <rdfs:domain rdf:resource="https://www.wikidata.org/wiki/Q617332"/>
        <rdfs:domain rdf:resource="https://www.wikidata.org/wiki/Q95074"/>
        <rdfs:range rdf:resource="https://purl.org/samcore#Trope"/>
        <rdfs:comment>This property relates a Story or a Scene to a Trope.</rdfs:comment>
        <rdfs:label>has trope</rdfs:label>
    </owl:ObjectProperty>
    


    <!-- https://purl.org/samcore#referenceMaterial -->

    <owl:ObjectProperty rdf:about="https://purl.org/samcore#referenceMaterial">
        <rdfs:domain rdf:resource="https://purl.org/samcore#Scene"/>
        <rdfs:range rdf:resource="https://www.wikidata.org/wiki/Q1385610"/>
        <rdfs:comment>This property connects a Scene to the Excerpt that is used as base to describe
            it.</rdfs:comment>
        <rdfs:label>reference material</rdfs:label>
        <rdfs:seeAlso>https://www.wikidata.org/wiki/Property:P144</rdfs:seeAlso>
    </owl:ObjectProperty>
    


    <!-- https://purl.org/samcore/relationship -->

    <owl:ObjectProperty rdf:about="https://purl.org/samcore/relationship">
        <rdfs:domain rdf:resource="https://www.wikidata.org/wiki/Q95074"/>
        <rdfs:range rdf:resource="https://www.wikidata.org/wiki/Q95074"/>
        <rdfs:comment>This is a placeholder property, it is preferable to use any property from
            &quot;https://vocab.org/relationship/rel-vocab-20100607.rdf&quot;.</rdfs:comment>
        <rdfs:label>relationship</rdfs:label>
    </owl:ObjectProperty>
    


    <!-- https://www.wikidata.org/wiki/Property:P106 -->

    <owl:ObjectProperty rdf:about="https://www.wikidata.org/wiki/Property:P106">
        <rdfs:domain rdf:resource="https://www.wikidata.org/wiki/Q95074"/>
        <rdfs:range rdf:resource="https://www.wikidata.org/wiki/Q12737077"/>
        <rdfs:comment>As described by Wikidata
            (&quot;https://www.wikidata.org/wiki/Property:P106&quot;), this property describes the
            occupation of a person.</rdfs:comment>
        <rdfs:label>occupation</rdfs:label>
    </owl:ObjectProperty>
    


    <!-- https://www.wikidata.org/wiki/Property:P1416 -->

    <owl:ObjectProperty rdf:about="https://www.wikidata.org/wiki/Property:P1416">
        <rdfs:domain rdf:resource="https://www.wikidata.org/wiki/Q12737077"/>
        <rdfs:range rdf:resource="https://purl.org/samcore#GroupOfCharacters"/>
        <rdfs:range rdf:resource="https://www.wikidata.org/wiki/Q43229"/>
        <rdfs:range rdf:resource="https://www.wikidata.org/wiki/Q95074"/>
        <rdfs:comment>As defined by Wikidata
            (&quot;https://www.wikidata.org/wiki/Property:P1416&quot;), this property connects to an
            organization that a person or organization is affiliated with (not necessarily member of
            or employed by).</rdfs:comment>
        <rdfs:label>affiliation</rdfs:label>
    </owl:ObjectProperty>
    


    <!-- https://www.wikidata.org/wiki/Property:P21 -->

    <owl:ObjectProperty rdf:about="https://www.wikidata.org/wiki/Property:P21">
        <rdfs:domain rdf:resource="https://www.wikidata.org/wiki/Q95074"/>
        <rdfs:range rdf:resource="https://sparql.cwrc.ca/ontologies/cwrc.html#Gender"/>
        <rdfs:comment>As described by Wikidata
            (&quot;https://www.wikidata.org/wiki/Property:P21&quot;) this property connects to the
            sex or gender identity of human or animal.</rdfs:comment>
        <rdfs:label>gender</rdfs:label>
    </owl:ObjectProperty>
    


    <!-- https://www.wikidata.org/wiki/Property:P2408 -->

    <owl:ObjectProperty rdf:about="https://www.wikidata.org/wiki/Property:P2408">
        <rdfs:domain rdf:resource="https://www.wikidata.org/wiki/Q617332"/>
        <rdfs:range rdf:resource="https://www.wikidata.org/wiki/Q6428674"/>
        <rdf:Description>As described by Wikidata (&quot;https://www.wikidata.org/wiki/Property:P2408&quot;), historical, contemporary, or future period, year, century or day the work or genre is set in or event featured in the story of the work</rdf:Description>
        <rdfs:label>set in period</rdfs:label>
    </owl:ObjectProperty>
    


    <!-- https://www.wikidata.org/wiki/Property:P2561 -->

    <owl:ObjectProperty rdf:about="https://www.wikidata.org/wiki/Property:P2561">
        <rdfs:domain rdf:resource="https://www.wikidata.org/wiki/Q95074"/>
        <rdfs:range rdf:resource="https://www.wikidata.org/wiki/Q82799"/>
        <rdfs:comment>As described by Wikidata
            (&quot;https://www.wikidata.org/wiki/Property:P2561&quot;), this property represents the
            name the subject is known by.</rdfs:comment>
        <rdfs:label>name</rdfs:label>
    </owl:ObjectProperty>
    


    <!-- https://www.wikidata.org/wiki/Property:P360 -->

    <owl:ObjectProperty rdf:about="https://www.wikidata.org/wiki/Property:P360">
        <rdfs:domain rdf:resource="https://purl.org/samcore#CharacterList"/>
        <rdfs:range rdf:resource="https://purl.org/samcore#GroupOfCharacters"/>
        <rdfs:range rdf:resource="https://www.wikidata.org/wiki/Q95074"/>
        <rdfs:comment>As described by Wikidata
            (&quot;https://www.wikidata.org/wiki/Property:P360&quot;), this property connects to a
            common element between all listed items.</rdfs:comment>
        <rdfs:label>is a list of</rdfs:label>
    </owl:ObjectProperty>
    


    <!-- https://www.wikidata.org/wiki/Property:P361 -->

    <owl:ObjectProperty rdf:about="https://www.wikidata.org/wiki/Property:P361">
        <owl:inverseOf rdf:resource="https://www.wikidata.org/wiki/Property:P527"/>
        <rdfs:domain rdf:resource="https://purl.org/samcore#Scene"/>
        <rdfs:domain rdf:resource="https://www.wikidata.org/wiki/Q95074"/>
        <rdfs:range rdf:resource="https://purl.org/samcore#GroupOfCharacters"/>
        <rdfs:range rdf:resource="https://purl.org/samcore#SequenceOfScenes"/>
        <rdfs:comment>As described by Wikidata
            (&quot;https://www.wikidata.org/wiki/Property:P361&quot;), this property connects to an
            object of which the subject is a part (if this subject is already part of object A which
            is a part of object B, then please only make the subject part of object A).</rdfs:comment>
        <rdfs:label>part of</rdfs:label>
    </owl:ObjectProperty>
    


    <!-- https://www.wikidata.org/wiki/Property:P3938 -->

    <owl:ObjectProperty rdf:about="https://www.wikidata.org/wiki/Property:P3938">
        <rdfs:domain rdf:resource="https://www.wikidata.org/wiki/Q82799"/>
        <rdfs:range>
            <owl:Class>
                <owl:unionOf rdf:parseType="Collection">
                    <rdf:Description rdf:about="https://purl.org/samcore#GroupOfCharacters"/>
                    <rdf:Description rdf:about="https://www.wikidata.org/wiki/Q43229"/>
                    <rdf:Description rdf:about="https://www.wikidata.org/wiki/Q95074"/>
                </owl:unionOf>
            </owl:Class>
        </rdfs:range>
        <rdfs:comment>As described by Wikidata
            (&quot;https://www.wikidata.org/wiki/Property:P3938&quot;), this property connects to the person or organisation that coined the name.</rdfs:comment>
        <rdfs:label>named by</rdfs:label>
    </owl:ObjectProperty>
    


    <!-- https://www.wikidata.org/wiki/Property:P527 -->

    <owl:ObjectProperty rdf:about="https://www.wikidata.org/wiki/Property:P527">
        <rdfs:domain rdf:resource="https://purl.org/samcore#Story"/>
        <rdfs:range rdf:resource="https://purl.org/samcore#CharacterList"/>
        <rdfs:range rdf:resource="https://purl.org/samcore#Scene"/>
        <rdfs:range rdf:resource="https://purl.org/samcore#SequenceOfScenes"/>
        <rdfs:comment>As described by Wikidata
            (&quot;https://www.wikidata.org/wiki/Property:P527&quot;), this property represents a
            part (or parts) of this subject.</rdfs:comment>
        <rdfs:label>has part(s)</rdfs:label>
    </owl:ObjectProperty>
    


    <!-- https://www.wikidata.org/wiki/Property:P625 -->

    <owl:ObjectProperty rdf:about="https://www.wikidata.org/wiki/Property:P625">
        <rdfs:domain rdf:resource="https://www.wikidata.org/wiki/Q17334923"/>
        <rdfs:range rdf:resource="https://www.wikidata.org/wiki/Q104224919"/>
        <rdfs:comment>As defined by Wikidata
            (&quot;https://www.wikidata.org/wiki/Property:P625&quot;), this property links to the
            geocoordinates of the subject.</rdfs:comment>
        <rdfs:label>coordinate location</rdfs:label>
    </owl:ObjectProperty>
    


    <!-- https://www.wikidata.org/wiki/Property:P7081 -->

    <owl:ObjectProperty rdf:about="https://www.wikidata.org/wiki/Property:P7081">
        <rdfs:domain rdf:resource="http://iflastandards.info/ns/lrm/lrmer/E4"/>
        <rdfs:range rdf:resource="https://www.wikidata.org/wiki/Q1385610"/>
        <rdfs:comment>As described by (&quot;https://www.wikidata.org/wiki/Property:P7081&quot;),
            &quot;quotation or excerpt from this work. No quotation marks needed&quot;. It is to be
            intended not as work, but Manifestation as Wikidata doesn&apos;t follow the FRBR model.</rdfs:comment>
        <rdfs:label>quotation or excerpt</rdfs:label>
    </owl:ObjectProperty>
    


    <!-- https://www.wikidata.org/wiki/Property:P710 -->

    <owl:ObjectProperty rdf:about="https://www.wikidata.org/wiki/Property:P710">
        <rdfs:domain rdf:resource="https://purl.org/samcore#Scene"/>
        <rdfs:domain rdf:resource="https://purl.org/samcore#Trope"/>
        <rdfs:domain rdf:resource="https://www.wikidata.org/wiki/Q1150070"/>
        <rdfs:range rdf:resource="https://purl.org/samcore#GroupOfCharacters"/>
        <rdfs:range rdf:resource="https://www.wikidata.org/wiki/Q95074"/>
        <rdfs:comment>As described by Wikidata
            (&quot;https://www.wikidata.org/wiki/Property:P710&quot;), this property identifies the
            person, group of people or organization (object) that actively takes/took part in an
            event or process (subject).</rdfs:comment>
        <rdfs:label>participant</rdfs:label>
    </owl:ObjectProperty>
    


    <!-- https://www.wikidata.org/wiki/Property:P8371 -->

    <owl:ObjectProperty rdf:about="https://www.wikidata.org/wiki/Property:P8371">
        <rdfs:domain rdf:resource="https://purl.org/samcore#Scene"/>
        <rdfs:domain rdf:resource="https://purl.org/samcore#Story"/>
        <rdfs:range rdf:resource="https://www.wikidata.org/wiki/Q96622155"/>
        <rdfs:comment>As described by Wikidata
            (&quot;https://www.wikidata.org/wiki/Property:P8371&quot;), this property connects to a
            creative work, tradition or theory this creative work references by allusion, quote or
            similar means.</rdfs:comment>
        <rdfs:label>references work, tradition or theory</rdfs:label>
    </owl:ObjectProperty>
    


    <!-- 
    ///////////////////////////////////////////////////////////////////////////////////////
    //
    // Data properties
    //
    ///////////////////////////////////////////////////////////////////////////////////////
     -->

    


    <!-- https://purl.org/samcore#changeExcerpt -->

    <owl:DatatypeProperty rdf:about="https://purl.org/samcore#changeExcerpt">
        <rdfs:domain rdf:resource="https://www.wikidata.org/wiki/Q1150070"/>
        <rdfs:range rdf:resource="http://www.w3.org/2000/01/rdf-schema#Literal"/>
        <rdfs:comment>This property is used to represent the literal value of a Change class if expressed through a string or referenced via an audiovisual timestamp.</rdfs:comment>
    </owl:DatatypeProperty>
    


    <!-- https://purl.org/samcore#date -->

    <owl:DatatypeProperty rdf:about="https://purl.org/samcore#date">
        <rdfs:domain rdf:resource="https://www.wikidata.org/wiki/Q12322185"/>
        <rdfs:range rdf:resource="http://www.w3.org/2001/XMLSchema#dateTime"/>
        <rdfs:comment>This property allows to register a point in time, inferred or given for a
            Setting entity.</rdfs:comment>
    </owl:DatatypeProperty>
    


    <!-- https://purl.org/samcore#descriptor -->

    <owl:DatatypeProperty rdf:about="https://purl.org/samcore#descriptor">
        <rdfs:domain rdf:resource="https://www.wikidata.org/wiki/Q95074"/>
        <rdfs:range rdf:resource="http://www.w3.org/2000/01/rdf-schema#Literal"/>
        <rdfs:comment>This property identifies a string as a &apos;Fictional Character&apos;
            descriptor, meaning that this string is recurrent and used to define the character in
            narration.</rdfs:comment>
    </owl:DatatypeProperty>
    


    <!-- https://purl.org/samcore#excerpt_text -->

    <owl:DatatypeProperty rdf:about="https://purl.org/samcore#excerpt_text">
        <rdfs:domain rdf:resource="https://www.wikidata.org/wiki/Q1385610"/>
        <rdfs:range rdf:resource="http://www.w3.org/2000/01/rdf-schema#Literal"/>
        <rdfs:comment>String for the corresponding Excerpt.</rdfs:comment>
        <rdfs:label>excerpt text</rdfs:label>
    </owl:DatatypeProperty>
    


    <!-- https://purl.org/samcore#hasName -->

    <owl:DatatypeProperty rdf:about="https://purl.org/samcore#hasName">
        <rdfs:domain rdf:resource="https://www.wikidata.org/wiki/Q82799"/>
        <rdfs:range rdf:resource="http://www.w3.org/2000/01/rdf-schema#Literal"/>
        <rdfs:comment>Name for the Name class, associated to a character</rdfs:comment>
    </owl:DatatypeProperty>
    


    <!-- https://purl.org/samcore#hasTitle -->

    <owl:DatatypeProperty rdf:about="https://purl.org/samcore#hasTitle">
        <rdfs:domain rdf:resource="https://www.wikidata.org/wiki/Q12737077"/>
        <rdfs:range rdf:resource="http://www.w3.org/2000/01/rdf-schema#Literal"/>
        <rdfs:comment>Current title for the occupation.</rdfs:comment>
    </owl:DatatypeProperty>
    


    <!-- https://purl.org/samcore#narratorName -->

    <owl:DatatypeProperty rdf:about="https://purl.org/samcore#narratorName">
        <rdfs:domain rdf:resource="https://www.wikidata.org/wiki/Q95074"/>
        <rdfs:range rdf:resource="http://www.w3.org/2000/01/rdf-schema#Literal"/>
        <rdfs:comment>A name assigned by the narrator to a character, used in third person narration
            when referring to the character, aside from his diegetical name(s). The narrator name
            can be used diegetically, but that must be tracked by the diegetical names attached to
            the character.</rdfs:comment>
        <rdfs:label>narratorName</rdfs:label>
    </owl:DatatypeProperty>
    


    <!-- https://purl.org/samcore#periodic_table -->

    <owl:DatatypeProperty rdf:about="https://purl.org/samcore#periodic_table">
        <rdfs:domain rdf:resource="https://purl.org/samcore#TvTropesTrope"/>
        <rdfs:range rdf:resource="http://www.w3.org/2001/XMLSchema#boolean"/>
        <rdfs:comment>True if the Trope is present on &quot;The Periodic Table of
            Storytelling&quot;, available at &quot;https://jamesharris.design/periodic&quot;</rdfs:comment>
    </owl:DatatypeProperty>
    


    <!-- https://purl.org/samcore#placeDescriptor -->

    <owl:DatatypeProperty rdf:about="https://purl.org/samcore#placeDescriptor">
        <rdfs:domain rdf:resource="https://www.wikidata.org/wiki/Q17334923"/>
        <rdfs:range rdf:resource="http://www.w3.org/2000/01/rdf-schema#Literal"/>
    </owl:DatatypeProperty>
    


    <!-- https://purl.org/samcore#referenceMaterialSource -->

    <owl:DatatypeProperty rdf:about="https://purl.org/samcore#referenceMaterialSource">
        <rdfs:domain rdf:resource="https://www.wikidata.org/wiki/Q1385610"/>
        <rdfs:range rdf:resource="http://www.w3.org/2000/01/rdf-schema#Literal"/>
        <rdfs:comment>This property allows to link to the resource that describes the reference material currently in use.</rdfs:comment>
        <rdfs:label>reference material source</rdfs:label>
    </owl:DatatypeProperty>
    


    <!-- https://purl.org/samcore#stringDate -->

    <owl:DatatypeProperty rdf:about="https://purl.org/samcore#stringDate">
        <rdfs:domain rdf:resource="https://www.wikidata.org/wiki/Q12322185"/>
        <rdfs:range rdf:resource="http://www.w3.org/2000/01/rdf-schema#Literal"/>
        <rdfs:comment>This data property allows the user to keep track of dates that don&apos;t
            follow a standard date format.</rdfs:comment>
    </owl:DatatypeProperty>
    


    <!-- https://purl.org/samcore#transition -->

    <owl:DatatypeProperty rdf:about="https://purl.org/samcore#transition">
        <rdfs:domain rdf:resource="https://purl.org/samcore#Scene"/>
        <rdfs:range rdf:resource="http://www.w3.org/2000/01/rdf-schema#Literal"/>
        <rdfs:comment>A word, sequence of words or timestamp that contains a clear transition from a
            scene to the other. This should be contained in the scene it helps transitioning to.</rdfs:comment>
    </owl:DatatypeProperty>
    


    <!-- https://purl.org/samcore#tropeURI -->

    <owl:DatatypeProperty rdf:about="https://purl.org/samcore#tropeURI">
        <rdfs:domain rdf:resource="https://purl.org/samcore#Trope"/>
        <rdfs:range rdf:resource="http://www.w3.org/2000/01/rdf-schema#Literal"/>
        <rdfs:comment>A URI leading to the relevant trope reference, the source of the trope may
            vary the domain of the URI.</rdfs:comment>
        <rdfs:label>tropeURI</rdfs:label>
    </owl:DatatypeProperty>
    


    <!-- 
    ///////////////////////////////////////////////////////////////////////////////////////
    //
    // Classes
    //
    ///////////////////////////////////////////////////////////////////////////////////////
     -->

    


    <!-- http://iflastandards.info/ns/lrm/lrmer/E4 -->

    <owl:Class rdf:about="http://iflastandards.info/ns/lrm/lrmer/E4">
        <rdfs:comment>As defined in LRMoo (&quot;https://www.iflastandards.info/lrm/lrmer#E4&quot;) this class represents a &quot;set of all carriers that are assumed to share the same characteristics as to intellectual or artistic content and aspects of physical form. That set is defined by both the overall content and the production plan for its carrier or carriers&quot;. It is necessary to have a Manifestation instead of an Expression or work because we can clearly reference, usually with timestamp and strings, to an existing product, improving accuracy. This class creates the entity that identify the portion and the manifestation the scene is attached to. This is necessary because the concept of Story by this model allows a scene to be shared by multiple manifestations.</rdfs:comment>
        <rdfs:label>Manifestation</rdfs:label>
    </owl:Class>
    


    <!-- https://purl.org/samcore#CharacterList -->

    <owl:Class rdf:about="https://purl.org/samcore#CharacterList">
        <rdfs:comment>This class collects all the characters and group of characters.</rdfs:comment>
        <rdfs:label>Character List</rdfs:label>
    </owl:Class>
    


    <!-- https://purl.org/samcore#GroupOfCharacters -->

    <owl:Class rdf:about="https://purl.org/samcore#GroupOfCharacters">
        <rdfs:comment>This class represents group of characters that are diegetically or narratively distinct. They can be ethnic groups that are relevant to the story, fantasy races or groups of people acting together or sharing a common scene, like an angry mob or a Greek tragedy chorus.</rdfs:comment>
        <rdfs:label>Group Of Characters</rdfs:label>
    </owl:Class>
    


    <!-- https://purl.org/samcore#PeriodicTableTrope -->

    <owl:Class rdf:about="https://purl.org/samcore#PeriodicTableTrope">
        <rdfs:subClassOf rdf:resource="https://purl.org/samcore#TvTropesTrope"/>
        <rdfs:comment>This class represent tropes selected by designer James Harris in his online tool &quot;The Periodic Table of Storytelling&quot;. The current url for the selection is at &quot;https://jamesharris.design/periodic/&quot;.</rdfs:comment>
        <rdfs:label>Periodic Table Trope</rdfs:label>
    </owl:Class>
    


    <!-- https://purl.org/samcore#Scene -->

    <owl:Class rdf:about="https://purl.org/samcore#Scene">
        <rdfs:comment>Any distinct unit of time and space, or significant change in characters and mood that is distinguished in the Story.</rdfs:comment>
        <rdfs:label>Scene</rdfs:label>
    </owl:Class>
    


    <!-- https://purl.org/samcore#SequenceOfScenes -->

    <owl:Class rdf:about="https://purl.org/samcore#SequenceOfScenes">
        <rdfs:comment>A coherent or strongly related sequence of scenes. This is usually called story arc, but it can also represent strong authorial choices in the structure of the story, therefore the collected scenes can be a part, or a chapter.</rdfs:comment>
        <rdfs:label>Group of Scenes</rdfs:label>
    </owl:Class>
    


    <!-- https://purl.org/samcore#Story -->

    <owl:Class rdf:about="https://purl.org/samcore#Story">
        <rdfs:comment>The vocabulary entry from wikidata in this case is unfitting. A narrative is described as the account of a series of events in written or oral form. In this model the intention is to abstract it from any constraint given by any form of expression, using it only as the source and reference to build the Story object, and disambiguating any definition that identify them as the same object.</rdfs:comment>
        <rdfs:label>Story</rdfs:label>
    </owl:Class>
    


    <!-- https://purl.org/samcore#Trope -->

    <owl:Class rdf:about="https://purl.org/samcore#Trope">
        <rdfs:comment>Any recognizable pattern recurring in Stories&apos; and their elements.</rdfs:comment>
        <rdfs:label>Trope</rdfs:label>
    </owl:Class>
    


    <!-- https://purl.org/samcore#TvTropesTrope -->

    <owl:Class rdf:about="https://purl.org/samcore#TvTropesTrope">
        <rdfs:subClassOf rdf:resource="https://purl.org/samcore#Trope"/>
        <rdfs:comment>A Trope defined by the online, crowd-sourced wiki &quot;https://tvtropes.org&quot;.</rdfs:comment>
        <rdfs:label>Tv Tropes Trope</rdfs:label>
    </owl:Class>
    


    <!-- https://sparql.cwrc.ca/ontologies/cwrc.html#Gender -->

    <owl:Class rdf:about="https://sparql.cwrc.ca/ontologies/cwrc.html#Gender">
        <rdfs:comment>As defined by the Canadian Writing Research Collaboratory Linked Open Data (&quot;https://sparql.cwrc.ca/ontologies/cwrc.html#Gender&quot;). this class represents a person&apos;s gender, whether attributed or self-reported, with accompanying context, where present, provided by gender context annotations. Although in popular culture gender and biological sex are conflated and understood to be binary, the concept of gender stresses the relationality, constructedness, and performativity of gendered identities and gendered behaviour, whose categories are historically contingent and the boundaries between them blurry.</rdfs:comment>
        <rdfs:label>Gender</rdfs:label>
    </owl:Class>
    


    <!-- https://www.wikidata.org/wiki/Q104224919 -->

    <owl:Class rdf:about="https://www.wikidata.org/wiki/Q104224919">
        <rdfs:comment>As defined by Wikidata (&quot;https://www.wikidata.org/wiki/Q104224919&quot;) this class represents a position on the Earth consisting of a latitude and a longitude.</rdfs:comment>
        <rdfs:label>Geographic Coordinates</rdfs:label>
    </owl:Class>
    


    <!-- https://www.wikidata.org/wiki/Q1150070 -->

    <owl:Class rdf:about="https://www.wikidata.org/wiki/Q1150070">
        <rdfs:subClassOf rdf:resource="https://www.wikidata.org/wiki/Q95074"/>
        <rdfs:comment>As defined by Wikidata (&quot;https://www.wikidata.org/wiki/Q1150070&quot;), change is a &quot;process, event or action that deviates from the present state&quot;. This class is set to be a node that should host any sort of character change.</rdfs:comment>
        <rdfs:label>Change</rdfs:label>
    </owl:Class>
    


    <!-- https://www.wikidata.org/wiki/Q12322185 -->

    <owl:Class rdf:about="https://www.wikidata.org/wiki/Q12322185">
        <rdfs:comment>As defined by Wikidata (https://www.wikidata.org/wiki/Q12322185) this class represents a designation of a point in time.</rdfs:comment>
        <rdfs:label>Time</rdfs:label>
    </owl:Class>
    


    <!-- https://www.wikidata.org/wiki/Q12737077 -->

    <owl:Class rdf:about="https://www.wikidata.org/wiki/Q12737077">
        <rdfs:comment>As defined by Wikidata (&quot;https://www.wikidata.org/wiki/Q12737077&quot;) this class represents a label applied to a person based on an activity they participate in.</rdfs:comment>
        <rdfs:label>Occupation</rdfs:label>
    </owl:Class>
    


    <!-- https://www.wikidata.org/wiki/Q1385610 -->

    <owl:Class rdf:about="https://www.wikidata.org/wiki/Q1385610">
        <rdfs:comment>As described by Wikidata (&quot;https://www.wikidata.org/wiki/Q1385610&quot;) &quot;an extract from a larger audiovisual or literary work&quot;, Excerpt is a class that describes the actual part of the reference Manifestation that the scene represents, allowing to keep track of the Manifestation and the sequence of characters or audio-visual units from which the scene is abstracted.</rdfs:comment>
        <rdfs:label>Excerpt</rdfs:label>
    </owl:Class>
    


    <!-- https://www.wikidata.org/wiki/Q17334923 -->

    <owl:Class rdf:about="https://www.wikidata.org/wiki/Q17334923">
        <rdfs:comment>As defined by Wikidata (https://www.wikidata.org/wiki/Q17334923) this class represents a &apos;property describing the position of something in space&apos;.</rdfs:comment>
        <rdfs:label>Physical Location</rdfs:label>
    </owl:Class>
    


    <!-- https://www.wikidata.org/wiki/Q43229 -->

    <owl:Class rdf:about="https://www.wikidata.org/wiki/Q43229">
        <rdfs:subClassOf rdf:resource="https://purl.org/samcore#GroupOfCharacters"/>
        <rdfs:comment>As defined by Wikidata (&quot;https://www.wikidata.org/wiki/Q43229&quot;) this class represents social entity established to meet needs or pursue goals.</rdfs:comment>
        <rdfs:label>Organisation</rdfs:label>
    </owl:Class>
    


    <!-- https://www.wikidata.org/wiki/Q617332 -->

    <owl:Class rdf:about="https://www.wikidata.org/wiki/Q617332">
        <rdfs:comment>As defined by Wikidata (https://www.wikidata.org/wiki/Q617332) this class represents a time and place within a narrative, whether fiction or non-fiction.</rdfs:comment>
        <rdfs:label>Setting</rdfs:label>
    </owl:Class>
    


    <!-- https://www.wikidata.org/wiki/Q6428674 -->

    <owl:Class rdf:about="https://www.wikidata.org/wiki/Q6428674">
        <rdf:Description>As descibed by Wikidata (&quot;https://www.wikidata.org/wiki/Property:P2348&quot;), time period (historic period or era, sports season, theatre season, legislative period etc.) in which the subject occurred or with which it is associated</rdf:Description>
        <rdfs:label>Era</rdfs:label>
    </owl:Class>
    


    <!-- https://www.wikidata.org/wiki/Q82799 -->

    <owl:Class rdf:about="https://www.wikidata.org/wiki/Q82799">
        <rdfs:comment>As defined by Wikidata (&quot;https://www.wikidata.org/wiki/Q82799&quot;) This class represents a word or phrase used for identification.</rdfs:comment>
        <rdfs:label>Name</rdfs:label>
    </owl:Class>
    


    <!-- https://www.wikidata.org/wiki/Q95074 -->

    <owl:Class rdf:about="https://www.wikidata.org/wiki/Q95074">
        <rdfs:comment>As defined by Wikidata (&quot;https://www.wikidata.org/wiki/Q95074&quot;) a class representing a fictional human or non-human character in a narrative work of art.</rdfs:comment>
        <rdfs:label>Fictional Character</rdfs:label>
    </owl:Class>
    


    <!-- https://www.wikidata.org/wiki/Q96622155 -->

    <owl:Class rdf:about="https://www.wikidata.org/wiki/Q96622155">
        <rdfs:comment>As described by Wikidata (&quot;https://www.wikidata.org/wiki/Q96622155&quot;), this class represents a reference to another work.</rdfs:comment>
        <rdfs:label>Reference</rdfs:label>
    </owl:Class>
    <rdf:Description>
        <rdf:Description></rdf:Description>
    </rdf:Description>
</rdf:RDF>



<!-- Generated by the OWL API (version 4.5.29.2024-05-13T12:11:03Z) https://github.com/owlcs/owlapi -->

